ironfleet/src/Dafny/Distributed/Impl/RSL/AppInterface.i.dfy
@@ -7,6 +7,7 @@ include "../Common/NodeIdentity.i.dfy"
 include "../../Services/RSL/AppStateMachine.i.dfy"
 
 module LiveRSL__AppInterface_i {
+import opened Native__Io_s
 import opened Native__NativeTypes_s
 import opened Collections__Maps_i
 import opened LiveRSL__Configuration_i
@@ -15,190 +16,503 @@ import opened LiveRSL__Types_i
 import opened Common__GenericMarshalling_i
 import opened Common__NodeIdentity_i
 import opened AppStateMachine_i
-
-type CAppState = uint64
-
-datatype CAppMessage = CAppIncrement() | CAppReply(response:uint64) | CAppInvalid()
-
-////////////////////////////////////////////////
-//      CAppState
-////////////////////////////////////////////////
-
-predicate CAppStateIsAbstractable(appstate:CAppState)
-{
-  true
-}
-
-function AbstractifyCAppStateToAppState(appstate:CAppState) : AppState
-  requires CAppStateIsAbstractable(appstate)
-{
-  appstate
-}
-
-function {:opaque} AbstractifyCAppStateSeqToAppStateSeq(s:seq<CAppState>) : seq<AppState>
-  requires forall i :: i in s ==> CAppStateIsAbstractable(i)
-  ensures |AbstractifyCAppStateSeqToAppStateSeq(s)| == |s|
-  ensures forall i :: 0 <= i < |AbstractifyCAppStateSeqToAppStateSeq(s)| ==> AbstractifyCAppStateSeqToAppStateSeq(s)[i] == AbstractifyCAppStateToAppState(s[i])
-{
-  if |s| == 0 then
-    []
-  else
-    [AbstractifyCAppStateToAppState(s[0])] + AbstractifyCAppStateSeqToAppStateSeq(s[1..])
-}
-
-
-/////////////  CAppState parsing and marshalling
-
-function method CAppState_grammar() : G { GUint64 }
-
-function method parse_AppState(val:V) : CAppState
-  requires ValInGrammar(val, CAppState_grammar())
-  ensures  CAppStateIsAbstractable(parse_AppState(val))
-{
-  val.u as CAppState
-}
-
-function method AppStateMarshallable(msg:CAppState) : bool
-{
-  true
-}
-
-method MarshallAppState(c:CAppState) returns (val:V)
-  requires AppStateMarshallable(c)
-  ensures  ValInGrammar(val, CAppState_grammar())
-  ensures  ValidVal(val)
-  ensures  parse_AppState(val) == c
-{
-  val := VUint64(c);
-}
-
-function max_app_state_size():int { 0x8000 } // 2^15  // 0xFEFF_FFCF_FFFF_FF00
-
-
-lemma lemma_AppStateBound(c:CAppState, val:V)
-  requires ValInGrammar(val, CAppState_grammar())
-  requires ValidVal(val)
-  requires parse_AppState(val) == c
-  ensures  SizeOfV(val) < max_app_state_size()
-{
-}
+import opened Math__mul_nonlinear_i
+import opened Math__mul_i
 
 ////////////////////////////////////////////////
 //      CAppMessage
 ////////////////////////////////////////////////
 
-// These trivial definitions are included here, since these functions
-// should be part of our interface with the app.  Future apps may have
-// more complex requirements
+datatype CAppMessage = CAppInvalid()
+                     | CAppGetRequest(key: Bytes)
+                     | CAppGetFoundReply(value: Bytes)
+                     | CAppGetUnfoundReply()
+                     | CAppSetRequest(key: Bytes, value: Bytes)
+                     | CAppSetSuccessReply()
+                     | CAppSetFailureReply()
+                     | CAppDeleteRequest(key: Bytes)
+                     | CAppDeleteFoundReply()
+                     | CAppDeleteUnfoundReply()
 
-predicate method ValidAppMessage(c:CAppMessage)
-{
-  true
-}
+// This trivial definition is included here, since it should be part
+// of our interface with the app.  Future apps may have more complex
+// requirements for abstractability.
 
 predicate CAppMessageIsAbstractable(c:CAppMessage)
 {
   true
 }
 
+predicate method ValidCAppMessage(c:CAppMessage)
+{
+  match c
+    case CAppInvalid()              => true
+    case CAppGetRequest(key)        => |key| <= MaxKeySize()
+    case CAppGetFoundReply(value)   => |value| <= MaxValueSize()
+    case CAppGetUnfoundReply()      => true
+    case CAppSetRequest(key, value) => |key| <= MaxKeySize() && |value| <= MaxValueSize()
+    case CAppSetSuccessReply()      => true
+    case CAppSetFailureReply()      => true
+    case CAppDeleteRequest(key)     => |key| <= MaxKeySize()
+    case CAppDeleteFoundReply()     => true
+    case CAppDeleteUnfoundReply()   => true
+}
+
 function AbstractifyCAppMessageToAppMessage(c:CAppMessage) : AppMessage
   requires CAppMessageIsAbstractable(c)
 {
   match c {
-    case CAppIncrement => AppIncrementRequest()
-    case CAppReply(response) => AppIncrementReply(response)
-    case CAppInvalid => AppInvalidReply()
+    case CAppInvalid() => AppInvalidMessage()
+    case CAppGetRequest(key) => AppGetRequest(key)
+    case CAppGetFoundReply(value) => AppGetFoundReply(value)
+    case CAppGetUnfoundReply() => AppGetUnfoundReply()
+    case CAppSetRequest(key, value) => AppSetRequest(key, value)
+    case CAppSetSuccessReply() => AppSetSuccessReply()
+    case CAppSetFailureReply() => AppSetFailureReply()
+    case CAppDeleteRequest(key) => AppDeleteRequest(key)
+    case CAppDeleteFoundReply() => AppDeleteFoundReply()
+    case CAppDeleteUnfoundReply() => AppDeleteUnfoundReply()
   }
 }
 
 /////////////  CAppMessage parsing and marshalling
 
-function method CAppMessage_grammar() : G { GTaggedUnion([GTuple([]), GUint64, GTuple([])]) }
+function method CAppMessage_grammar() : G { GTaggedUnion([
+  GTuple([]),                       // CAppInvalid
+  GByteArray,                       // CAppGetRequest
+  GByteArray,                       // CAppGetFoundReply
+  GTuple([]),                       // CAppGetUnfoundReply
+  GTuple([GByteArray, GByteArray]), // CAppSetRequest
+  GTuple([]),                       // CAppSetSuccessReply
+  GTuple([]),                       // CAppSetFailureReply
+  GByteArray,                       // CAppDeleteRequest
+  GTuple([]),                       // CAppDeleteFoundReply
+  GTuple([])                        // CAppDeleteUnfoundReply
+]) }
 
 function method parse_AppMessage(val:V) : CAppMessage
   requires ValInGrammar(val, CAppMessage_grammar())
 {
   if val.c == 0 then
-    CAppIncrement()
+    CAppInvalid()
   else if val.c == 1 then
     assert ValInGrammar(val.val, CAppMessage_grammar().cases[1]);
-    CAppReply(val.val.u)
+    CAppGetRequest(val.val.b)
+  else if val.c == 2 then
+    assert ValInGrammar(val.val, CAppMessage_grammar().cases[2]);
+    CAppGetFoundReply(val.val.b)
+  else if val.c == 3 then
+    assert ValInGrammar(val.val, CAppMessage_grammar().cases[3]);
+    CAppGetUnfoundReply()
+  else if val.c == 4 then
+    assert ValInGrammar(val.val, CAppMessage_grammar().cases[4]);
+    CAppSetRequest(val.val.t[0].b, val.val.t[1].b)
+  else if val.c == 5 then
+    assert ValInGrammar(val.val, CAppMessage_grammar().cases[5]);
+    CAppSetSuccessReply()
+  else if val.c == 6 then
+    assert ValInGrammar(val.val, CAppMessage_grammar().cases[6]);
+    CAppSetFailureReply()
+  else if val.c == 7 then
+    assert ValInGrammar(val.val, CAppMessage_grammar().cases[7]);
+    CAppDeleteRequest(val.val.b)
+  else if val.c == 8 then
+    assert ValInGrammar(val.val, CAppMessage_grammar().cases[8]);
+    CAppDeleteFoundReply()
+  else if val.c == 9 then
+    assert ValInGrammar(val.val, CAppMessage_grammar().cases[9]);
+    CAppDeleteUnfoundReply()
   else
-    assert val.c == 2;
     CAppInvalid()
 }
 
 method MarshallCAppMessage(c:CAppMessage) returns (val:V)
   requires CAppMessageIsAbstractable(c)
-  requires ValidAppMessage(c)
+  requires ValidCAppMessage(c)
   ensures  ValInGrammar(val, CAppMessage_grammar())
   ensures  ValidVal(val)
   ensures  parse_AppMessage(val) == c
 {
   match c {
-    case CAppIncrement       => val := VCase(0, VTuple([]));
-    case CAppReply(response) => val := VCase(1, VUint64(response));
-    case CAppInvalid         => val := VCase(2, VTuple([]));
+    case CAppInvalid()              => val := VCase(0, VTuple([]));
+    case CAppGetRequest(key)        => val := VCase(1, VByteArray(key));
+    case CAppGetFoundReply(value)   => val := VCase(2, VByteArray(value));
+    case CAppGetUnfoundReply()      => val := VCase(3, VTuple([]));
+
+    case CAppSetRequest(key, value) =>
+      val := VCase(4, VTuple([VByteArray(key), VByteArray(value)]));
+      ghost var g := CAppMessage_grammar();
+      assert |val.val.t| == 2 == |g.cases[4].t|;
+      forall i | 0 <= i < |val.val.t|
+        ensures ValInGrammar(val.val.t[i], g.cases[4].t[i])
+        ensures ValidVal(val.val.t[i])
+      {
+        if i == 0 { } else if i == 1 { } else { assert false; }
+      }
+
+    case CAppSetSuccessReply()      => val := VCase(5, VTuple([]));
+    case CAppSetFailureReply()      => val := VCase(6, VTuple([]));
+    case CAppDeleteRequest(key)     => val := VCase(7, VByteArray(key));
+    case CAppDeleteFoundReply()     => val := VCase(8, VTuple([]));
+    case CAppDeleteUnfoundReply()   => val := VCase(9, VTuple([]));
   }
 }
 
-function method max_val_len() : int { 64 }  //{ 0x100_0000 }    // 2^24
-
+function method max_val_len() : int { MaxKeySize() + MaxValueSize() + 25 }
 
 lemma lemma_AppMessageBound(c:CAppMessage, val:V)
   requires ValInGrammar(val, CAppMessage_grammar())
-  requires ValidAppMessage(c)
+  requires ValidCAppMessage(c)
   requires parse_AppMessage(val) == c
   ensures  ValidVal(val)
-  ensures  SizeOfV(val) < max_val_len()   // 0x100_0000; // 2^24
+  ensures  SizeOfV(val) < max_val_len()
 {
-  forall ensures SeqSum([]) == 0
-  {
-    reveal SeqSum();
+  assert SeqSum([]) == 0 by { reveal SeqSum(); }
+
+  match c {
+    case CAppInvalid() =>
+      assert SizeOfV(val) == 8;
+
+    case CAppGetRequest(key) =>
+      assert SizeOfV(val) <= 16 + MaxKeySize();
+      
+    case CAppGetFoundReply(value) =>
+      assert SizeOfV(val) <= 16 + MaxValueSize();
+
+    case CAppGetUnfoundReply() =>
+      assert SizeOfV(val) == 8;
+
+    case CAppSetRequest(key, value) =>
+      ghost var g := CAppMessage_grammar();
+      assert ValInGrammar(val.val, g.cases[4]);
+      assert |val.val.t| == |g.cases[4].t| == 2;
+      assert val.val.t[0].b == key;
+      assert val.val.t[1].b == value;
+      assert val.val.t[2..] == [];
+      assert forall v :: v in val.val.t ==> ValidVal(v);
+      calc {
+        SizeOfV(val);
+        8 + SizeOfV(val.val);
+        8 + SeqSum(val.val.t);
+          { reveal SeqSum(); }
+        8 + (SizeOfV(val.val.t[0]) + SeqSum(val.val.t[1..]));
+          { reveal SeqSum(); }
+        8 + (SizeOfV(val.val.t[0]) + (SizeOfV(val.val.t[1]) + SeqSum(val.val.t[2..])));
+        8 + SizeOfV(val.val.t[0]) + SizeOfV(val.val.t[1]);
+        <= { assert |val.val.t[0].b| <= MaxKeySize(); }
+          8 + (8 + MaxKeySize()) + SizeOfV(val.val.t[1]);
+        <= { assert |val.val.t[1].b| <= MaxValueSize(); }
+          8 + (8 + MaxKeySize()) + (8 + MaxValueSize());
+        MaxKeySize() + MaxValueSize() + 24;
+      }
+
+    case CAppSetSuccessReply() =>
+      assert SizeOfV(val) == 8;
+
+    case CAppSetFailureReply() =>
+      assert SizeOfV(val) == 8;
+
+    case CAppDeleteRequest(key) =>
+      assert SizeOfV(val) <= 16 + MaxKeySize();
+
+    case CAppDeleteFoundReply() =>
+      assert SizeOfV(val) == 8;
+
+    case CAppDeleteUnfoundReply() =>
+      assert SizeOfV(val) == 8;
   }
 }
 
+////////////////////////////////////////////////
+//     CAppState (App State Machine)
+////////////////////////////////////////////////
 
-////////////////////////////////////////////////
-//     App State Machine 
-////////////////////////////////////////////////
+type CAppState = MutableMap<Bytes, Bytes>
+
+predicate CAppStateIsAbstractable(appstate: CAppState)
+{
+  true
+}
+
+function AbstractifyCAppStateToAppState(appstate: CAppState) : AppState
+  reads appstate
+  requires CAppStateIsAbstractable(appstate)
+{
+  MutableMap.MapOf(appstate)
+}
+
+predicate AppStateMarshallable(c:CAppState)
+  reads c
+{
+  var m := MutableMap.MapOf(c);
+  && |m.Keys| <= MaxNumKeys()
+  && (forall k :: k in m.Keys ==> |k| <= MaxKeySize() && |m[k]| <= MaxValueSize())
+}
 
 method CAppState_Init() returns (s:CAppState)
   ensures CAppStateIsAbstractable(s)
   ensures AbstractifyCAppStateToAppState(s) == AppInitialize()
   ensures AppStateMarshallable(s)
 {
-  s := 0;
+  s := MutableMap.EmptyMap();
 }
 
-
-method CappedIncrImpl(v:uint64) returns (v':uint64)
-  requires 0 <= v <= 0xffff_ffff_ffff_ffff
-  ensures v' == CappedIncr(v)
+method HandleAppGetRequest(appState:CAppState, key:Bytes) returns (reply:CAppMessage)
+  requires CAppStateIsAbstractable(appState)
+  requires AppStateMarshallable(appState)
+  ensures  CAppMessageIsAbstractable(reply)
+  ensures  AppHandleRequest(AbstractifyCAppStateToAppState(appState), AbstractifyCAppMessageToAppMessage(CAppGetRequest(key))) ==
+             (AbstractifyCAppStateToAppState(appState), AbstractifyCAppMessageToAppMessage(reply))
+  ensures  ValidCAppMessage(reply)
 {
-  if (v == 0xffff_ffff_ffff_ffff) {
-    v' := v;
-  } else {
-    v' := v + 1;
+  var contains, value := appState.TryGetValue(key);
+  if !contains {
+    reply := CAppGetUnfoundReply();
+  }
+  else {
+    reply := CAppGetFoundReply(value);
   }
 }
 
-method HandleAppRequest(appState:CAppState, request:CAppMessage) returns (appState':CAppState, reply:CAppMessage)
+method HandleAppSetRequest(appState:CAppState, key:Bytes, value:Bytes) returns (reply:CAppMessage)
+  modifies appState
+  requires CAppStateIsAbstractable(appState)
+  requires AppStateMarshallable(appState)
+  ensures  CAppStateIsAbstractable(appState)
+  ensures  CAppMessageIsAbstractable(reply)
+  ensures  AppStateMarshallable(appState)
+  ensures  AppHandleRequest(old(AbstractifyCAppStateToAppState(appState)), AbstractifyCAppMessageToAppMessage(CAppSetRequest(key, value)))
+             == (AbstractifyCAppStateToAppState(appState), AbstractifyCAppMessageToAppMessage(reply))
+  ensures  ValidCAppMessage(reply)
+{
+  if |key| > MaxKeySize() {
+    reply := CAppSetFailureReply();
+    return;
+  }
+
+  if |value| > MaxValueSize() {
+    reply := CAppSetFailureReply();
+    return;
+  }
+  
+  var sz := appState.Size();
+  assert sz <= MaxNumKeys();
+
+  // If the maximum number of keys has already been reached and we're supposed to
+  // set a key that isn't present, then do nothing but return a failure reply,
+  // so that we don't exceed the maximum number of keys allowed.  This behavior
+  // is what the spec specifies.
+
+  if sz == MaxNumKeys() {
+    var contains := appState.Contains(key);
+    if !contains {
+      reply := CAppSetFailureReply();
+      return;
+    }
+  }
+
+  appState.Set(key, value);
+  reply := CAppSetSuccessReply();
+}
+
+method HandleAppDeleteRequest(appState:CAppState, key:Bytes) returns (reply:CAppMessage)
+  modifies appState
+  requires CAppStateIsAbstractable(appState)
+  requires AppStateMarshallable(appState)
+  ensures  CAppStateIsAbstractable(appState)
+  ensures  CAppMessageIsAbstractable(reply)
+  ensures  AppStateMarshallable(appState)
+  ensures  AppHandleRequest(old(AbstractifyCAppStateToAppState(appState)), AbstractifyCAppMessageToAppMessage(CAppDeleteRequest(key))) ==
+             (AbstractifyCAppStateToAppState(appState), AbstractifyCAppMessageToAppMessage(reply))
+  ensures  ValidCAppMessage(reply)
+{
+  var contains := appState.Contains(key);
+  if contains {
+    appState.Remove(key);
+    reply := CAppDeleteFoundReply();
+  }
+  else {
+    reply := CAppDeleteUnfoundReply();
+  }
+}
+
+method HandleAppRequest(appState:CAppState, request:CAppMessage) returns (reply:CAppMessage)
+  modifies appState
   requires CAppStateIsAbstractable(appState)
   requires CAppMessageIsAbstractable(request)
-  ensures  CAppStateIsAbstractable(appState')
+  requires AppStateMarshallable(appState)
+  ensures  CAppStateIsAbstractable(appState)
   ensures  CAppMessageIsAbstractable(reply)
-  ensures  AppStateMarshallable(appState')
-  ensures  AppHandleRequest(AbstractifyCAppStateToAppState(appState), AbstractifyCAppMessageToAppMessage(request)) == 
-             (AbstractifyCAppStateToAppState(appState'), AbstractifyCAppMessageToAppMessage(reply))
+  ensures  AppStateMarshallable(appState)
+  ensures  AppHandleRequest(old(AbstractifyCAppStateToAppState(appState)), AbstractifyCAppMessageToAppMessage(request)) ==
+             (AbstractifyCAppStateToAppState(appState), AbstractifyCAppMessageToAppMessage(reply))
+  ensures  ValidCAppMessage(reply)
 {
-  if request.CAppIncrement? {
-    appState' := CappedIncrImpl(appState);
-    reply := CAppReply(appState');
-  } else {
-    appState' := appState;
-    reply := CAppInvalid();
+  match request {
+    case CAppGetRequest(key) =>
+      reply := HandleAppGetRequest(appState, key);
+
+    case CAppSetRequest(key, value) =>
+      reply := HandleAppSetRequest(appState, key, value);
+
+    case CAppDeleteRequest(key) =>
+      reply := HandleAppDeleteRequest(appState, key);
+
+    case _ =>
+      reply := CAppInvalid();
   }
+}
+
+////////////////////////////////////////////////
+//      CTransferableAppState
+////////////////////////////////////////////////
+
+type CTransferableAppState = seq<(Bytes, Bytes)>
+
+predicate CTransferableAppStateIsAbstractable(appstate: CTransferableAppState)
+{
+  true
+}
+
+function AbstractifyCTransferableAppStateToAppState(appstate: CTransferableAppState) : AppState
+  requires CTransferableAppStateIsAbstractable(appstate)
+{
+  KVTupleSeqToMap(appstate)
+}
+
+/////////////  CTransferableAppState parsing and marshalling
+
+function method CTransferableAppState_grammar() : G
+{
+  GArray(GTuple([GByteArray, GByteArray]))
+}
+
+function method parse_KVTuple(val: V) : (Bytes, Bytes)
+  requires ValInGrammar(val, GTuple([GByteArray, GByteArray]))
+{
+  ghost var g := GTuple([GByteArray, GByteArray]);
+  assert ValInGrammar(val.t[0], g.t[0]);
+  assert ValInGrammar(val.t[1], g.t[1]);
+  (val.t[0].b, val.t[1].b)
+}
+
+function method parse_KVTupleSeq(vals: seq<V>) : (result: seq<(Bytes, Bytes)>)
+  requires forall val :: val in vals ==> ValInGrammar(val, GTuple([GByteArray, GByteArray]))
+  ensures  |result| == |vals|
+  ensures  forall i :: 0 <= i < |vals| ==> result[i] == parse_KVTuple(vals[i])
+{
+  if |vals| == 0 then
+    []
+  else
+    [parse_KVTuple(vals[0])] + parse_KVTupleSeq(vals[1..])
+}
+
+function method parse_TransferableAppState(val:V) : CTransferableAppState
+  requires ValInGrammar(val, CTransferableAppState_grammar())
+  ensures  CTransferableAppStateIsAbstractable(parse_TransferableAppState(val))
+{
+  parse_KVTupleSeq(val.a)
+}
+
+function method TransferableAppStateMarshallable(c:CTransferableAppState) : bool
+{
+  && |c| <= MaxNumKeys()
+  && (forall kv :: kv in c ==> |kv.0| <= MaxKeySize() && |kv.1| <= MaxValueSize())
+}
+
+function max_transferable_app_state_size():int { 0x1000_0000_0000_0000 } // 2^60
+
+lemma lemma_SeqSumMultiply(vals: seq<V>, bound: int)
+  requires forall val :: val in vals ==> SizeOfV(val) <= bound
+  ensures SeqSum(vals) <= bound * |vals|
+{
+  reveal SeqSum();
+  if |vals| == 0 {
+    return;
+  }
+  lemma_SeqSumMultiply(vals[1..], bound);
+  calc {
+    SeqSum(vals);
+    SizeOfV(vals[0]) + SeqSum(vals[1..]);
+    <= bound + SeqSum(vals[1..]);
+    <= bound + bound * |vals[1..]|;
+    bound + bound * (|vals| - 1);
+    bound * 1 + bound * (|vals| - 1);
+      { lemma_mul_is_distributive_add(bound, 1, |vals| - 1); }
+     bound * (1 + (|vals| - 1));
+     bound * |vals|;
+  }
+}
+
+lemma lemma_TransferableAppStateBound(c:CTransferableAppState, val:V)
+  requires ValInGrammar(val, CTransferableAppState_grammar())
+  requires ValidVal(val)
+  requires parse_TransferableAppState(val) == c
+  requires TransferableAppStateMarshallable(c)
+  ensures  SizeOfV(val) < max_transferable_app_state_size()
+{
+  var bound := MaxKeySize() + MaxValueSize() + 16;
+
+  forall v | v in val.a
+    ensures SizeOfV(v) <= bound
+  {
+    assert ValInGrammar(v, GTuple([GByteArray, GByteArray]));
+    assert |v.t| == 2;
+    assert |v.t[0].b| <= MaxKeySize();
+    assert |v.t[1].b| <= MaxValueSize();
+    reveal SeqSum();
+    calc {
+      SizeOfV(v);
+      SeqSum(v.t);
+      SizeOfV(v.t[0]) + (SizeOfV(v.t[1]) + SeqSum(v.t[1+1..]));
+      SizeOfV(v.t[0]) + SizeOfV(v.t[1]);
+      <= (8 + MaxKeySize()) + SizeOfV(v.t[1]);
+      <= (8 + MaxKeySize()) + (8 + MaxValueSize());
+      MaxKeySize() + MaxValueSize() + 16;
+      bound;
+    }
+  }
+
+  calc {
+    SizeOfV(val);
+    8 + SeqSum(val.a);
+    <= { lemma_SeqSumMultiply(val.a, bound); }
+      8 + bound * |val.a|;
+    <= { lemma_mul_is_commutative(bound, |val.a|);
+        lemma_mul_is_commutative(bound, MaxNumKeys());
+        lemma_mul_inequality(|val.a|, MaxNumKeys(), bound); }
+      8 + bound * MaxNumKeys();
+    < max_transferable_app_state_size();
+  }
+}
+
+method MarshallTransferableAppState(c:CTransferableAppState) returns (val:V)
+  requires TransferableAppStateMarshallable(c)
+  ensures  ValInGrammar(val, CTransferableAppState_grammar())
+  ensures  ValidVal(val)
+  ensures  parse_TransferableAppState(val) == c
+{
+  var kvs: seq<V> := [];
+  var i: int := 0;
+  while i < |c|
+    invariant 0 <= i <= |c|
+    invariant |kvs| == i
+    invariant ValInGrammar(VArray(kvs), CTransferableAppState_grammar())
+    invariant forall v :: v in kvs ==> ValidVal(v)
+    invariant ValidVal(VArray(kvs))
+    invariant parse_TransferableAppState(VArray(kvs)) == c[..i]
+  {
+    var (k, v) := c[i];
+    var k' := VByteArray(k);
+    var v' := VByteArray(v);
+    var kv' := VTuple([k', v']);
+    assert ValidVal(kv');
+    assert ValInGrammar(kv', GTuple([GByteArray, GByteArray]));
+    kvs := kvs + [kv'];
+    i := i + 1;
+  }
+
+  val := VArray(kvs);
 }
 
 }
