ironfleet/src/Dafny/Distributed/Services/RSL/AppStateMachine.i.dfy
@@ -1,36 +1,111 @@
 include "AppStateMachine.s.dfy"
 
-module AppStateMachine_i refines AppStateMachine_s {
-type AppState = uint64
 
-datatype AppMessage' = AppIncrementRequest() | AppIncrementReply(response:uint64) | AppInvalidReply()
+module AppStateMachine_i refines AppStateMachine_s {
+type Bytes = seq<byte>
+type AppState = map<Bytes, Bytes>
+
+datatype AppMessage' = AppInvalidMessage()
+                     | AppGetRequest(key: Bytes)
+                     | AppGetFoundReply(value: Bytes)
+                     | AppGetUnfoundReply()
+                     | AppSetRequest(key: Bytes, value: Bytes)
+                     | AppSetSuccessReply()
+                     | AppSetFailureReply()
+                     | AppDeleteRequest(key: Bytes)
+                     | AppDeleteFoundReply()
+                     | AppDeleteUnfoundReply()
 type AppMessage = AppMessage'
 
-function AppInitialize() : AppState { 0 }
+function AppInitialize() : AppState { map [] }
 
-function CappedIncr(v:uint64) : uint64
+// We have to use RemoveElementFromMap to work around a bug in Dafny
+// that crashes it.  That bug manifests when you define a type T with
+// type T = map<...> and then subtract a set from something of type T.
+
+function RemoveElementFromMap(m: map<Bytes, Bytes>, s: Bytes) : map<Bytes, Bytes>
 {
-  if (v == 0xffff_ffff_ffff_ffff) then
-    v
-  else
-    v + 1
+  m - {s}
 }
 
-function AppHandleRequest(m:AppState, request:AppMessage) : (AppState, AppMessage)
+function AppHandleRequest(m: AppState, request: AppMessage) : (AppState, AppMessage)
 {
-  if request.AppIncrementRequest? then
-    (CappedIncr(m), AppIncrementReply(CappedIncr(m)))
-  else
-    (m, AppInvalidReply())
+  match request
+    case AppGetRequest(key) =>
+      (m, if key in m then AppGetFoundReply(m[key]) else AppGetUnfoundReply())
+
+    case AppSetRequest(key, value) =>
+      var m' := m[key := value];
+      if |m'.Keys| > MaxNumKeys() || |key| > MaxKeySize() || |value| > MaxValueSize() then
+        (m, AppSetFailureReply())
+      else
+        (m', AppSetSuccessReply())
+
+    case AppDeleteRequest(key) =>
+      if key in m then
+        (RemoveElementFromMap(m, key), AppDeleteFoundReply())
+      else
+        (m, AppDeleteUnfoundReply())
+
+    case _ =>
+      (m, AppInvalidMessage())
 }
 
-function MarshallAppMessage(m:AppMessage) : seq<byte>
+function method MaxKeySize() : int   { 0x10_0000 } // 1 MB
+function method MaxValueSize() : int { 0x800_0000 } // 128 MB
+function method MaxNumKeys() : int   { 0x1_0000_0000 } // 2^32
+
+predicate ValidAppMessage(m: AppMessage)
 {
-  match m {                             // Case                    // Payload
-    case AppIncrementRequest =>         [0, 0, 0, 0, 0, 0, 0, 0] 
-    case AppIncrementReply(response) => [0, 0, 0, 0, 0, 0, 0, 1] + Uint64ToBytes(response)
-    case AppInvalidReply =>             [0, 0, 0, 0, 0, 0, 0, 2] 
-  }
+  match m
+    case AppInvalidMessage() => false
+    case AppGetRequest(key) => |key| <= MaxKeySize()
+    case AppGetFoundReply(value) => |value| <= MaxValueSize()
+    case AppGetUnfoundReply() => true
+    case AppSetRequest(key, value) => |key| <= MaxKeySize() && |value| <= MaxValueSize()
+    case AppSetSuccessReply() => true
+    case AppSetFailureReply() => true
+    case AppDeleteRequest(key) => |key| <= MaxKeySize()
+    case AppDeleteFoundReply() => true
+    case AppDeleteUnfoundReply() => true
+}
+
+function MarshallAppMessage(m: AppMessage) : seq<byte>
+{
+  if ValidAppMessage(m) then
+    match m {
+      case AppInvalidMessage() =>
+        [0, 0, 0, 0, 0, 0, 0, 0]
+
+      case AppGetRequest(key) =>
+        [0, 0, 0, 0, 0, 0, 0, 1] + Uint64ToBytes(|key| as uint64) + key
+
+      case AppGetFoundReply(value) =>
+        [0, 0, 0, 0, 0, 0, 0, 2] + Uint64ToBytes(|value| as uint64) + value
+
+      case AppGetUnfoundReply() =>
+        [0, 0, 0, 0, 0, 0, 0, 3]
+
+      case AppSetRequest(key, value) =>
+        [0, 0, 0, 0, 0, 0, 0, 4] + Uint64ToBytes(|key| as uint64) + key + Uint64ToBytes(|value| as uint64) + value
+      
+      case AppSetSuccessReply() =>
+        [0, 0, 0, 0, 0, 0, 0, 5]
+      
+      case AppSetFailureReply() =>
+        [0, 0, 0, 0, 0, 0, 0, 6]
+      
+      case AppDeleteRequest(key) =>
+        [0, 0, 0, 0, 0, 0, 0, 7] + Uint64ToBytes(|key| as uint64) + key
+
+      case AppDeleteFoundReply() =>
+        [0, 0, 0, 0, 0, 0, 0, 8]
+
+      case AppDeleteUnfoundReply() =>
+        [0, 0, 0, 0, 0, 0, 0, 9]
+    }
+  else
+    [0, 0, 0, 0, 0, 0, 0, 0]
 }
 
 function Uint64ToBytes(u:uint64) : seq<byte>
