ironfleet/src/Dafny/Distributed/Common/Native/IoLemmas.i.dfy
@@ -1,0 +1,81 @@
+include "Io.s.dfy"
+
+module Native__IoLemmas_i {
+
+import opened Native__NativeTypes_s
+import opened Native__Io_s
+
+lemma lemma_KVTupleSeqToMapCantIncreaseNumKeys<K, V>(kvs: seq<(K, V)>)
+  ensures |KVTupleSeqToMap(kvs)| <= |kvs|
+{
+  if |kvs| == 0 {
+    return;
+  }
+
+  var kvs_prefix := kvs[..|kvs|-1];
+  lemma_KVTupleSeqToMapCantIncreaseNumKeys(kvs_prefix);
+}
+
+lemma lemma_SetOfSequenceElementsNoBiggerThanSeq<T>(s: seq<T>)
+  ensures |(set x | x in s)| <= |s|
+{
+  if |s| == 0 {
+    return;
+  }
+
+  lemma_SetOfSequenceElementsNoBiggerThanSeq(s[1..]);
+  assert (set x | x in s) == {s[0]} + (set x | x in s[1..]);
+}
+
+lemma lemma_AsKVTuplesEnsuresKeysDistinct<K, V>(m: map<K, V>, kvs: seq<(K, V)>)
+  requires |kvs| == |m.Keys|
+  requires forall k :: k in m ==> (k, m[k]) in kvs
+  requires forall k, v :: (k, v) in kvs ==> k in m && m[k] == v
+  requires |kvs| > 0
+  ensures  kvs[|kvs|-1] !in kvs[..|kvs|-1]
+{
+  forall kv | kv in kvs
+    ensures kv in m.Items
+  {
+    var (k, v) := kv;
+    assert k in m && m[k] == v;
+    assert kv in m.Items;
+  }
+
+  forall kv | kv in m.Items
+    ensures kv in kvs
+  {
+    var (k, v) := kv;
+    assert k in m && m[k] == v;
+    assert (k, m[k]) in kvs;
+  }
+
+  var kv_last := kvs[|kvs|-1];
+  var kvs_prefix := kvs[..|kvs|-1];
+  if kv_last in kvs_prefix {
+    var s'' := set kv | kv in kvs_prefix;
+    assert s'' == m.Items;
+    lemma_SetOfSequenceElementsNoBiggerThanSeq(kvs_prefix);
+    assert |s''| <= |kvs_prefix| < |kvs|;
+    assert false;
+  }
+}
+
+lemma lemma_AsKVTuplesThenKVTupleSeqToMapIsIdentity<K, V>(m: map<K, V>, kvs: seq<(K, V)>)
+  requires |kvs| == |m.Keys|
+  requires forall k :: k in m ==> (k, m[k]) in kvs
+  requires forall k, v :: (k, v) in kvs ==> k in m && m[k] == v
+  ensures  KVTupleSeqToMap(kvs) == m
+{
+  if |kvs| == 0 {
+    return;
+  }
+
+  var kvs_prefix := kvs[..|kvs|-1];
+  var kv_last := kvs[|kvs|-1];
+  var m_prefix := m - {kv_last.0};
+  assert kv_last !in kvs_prefix by { lemma_AsKVTuplesEnsuresKeysDistinct(m, kvs); }
+  lemma_AsKVTuplesThenKVTupleSeqToMapIsIdentity(m_prefix, kvs_prefix);
+}
+
+}
